code/Yazi.Tree.Types.fsti
@@ -50,6 +50,7 @@ type heap_internal_index_t (hl: heap_len_t) = i: U32.t{
   0 < U32.v i /\ U32.v i <= U32.v hl / 2
 }
 
+noextract
 type tree_len_t = tl: Ghost.erased nat{tl <= U32.v heap_size}
 
 type tree_depth_t = B.lbuffer U8.t (2 * U32.v l_codes + 1)
